domain and range argument ordering in index_map_spec

IndexFunctions.v
@@ -16,8 +16,13 @@ Global Open Scope nat_scope.
 (* Vector index mapping functon which maps between two sets of natrual
      numers. Mapping is partial and it returns None if there is no correspondance
      between a number in source set and target set. *)
-Definition index_map_spec (range domain : nat) :=
+Definition index_map_spec (domain range: nat) :=
   forall n : nat, n < domain -> {v : option nat | forall n' : nat, v ≡ Some n' -> n' < range}.
 
+(* Returns upper domain bound for given `index_map_spec` *)
+Definition index_map_dom {d r:nat} (s: index_map_spec d r) := d.
+
+(* Returns upper rang bound for given `index_map_spec` *)
+Definition index_map_range {d r:nat} (s: index_map_spec d r) := r.
 
 
